ExnTransformer: still working on applicative part

src/ExnTransformer.v
@@ -1,22 +1,83 @@
 Add LoadPath "./" as Monads .
+
 Require Import Monads.FunctorApplicativeMonad.
-Require Import Monads.ExnMonad.
-From Coq Require Import FunctionalExtensionality Program.Basics.
+
+From Coq Require Import FunctionalExtensionality Program.Basics String.
 Notation "x <- c1 ;; c2" := (bind c1 (fun x => c2)) 
                              (right associativity, at level 84, c1 at next level).
 
-Definition exn_t (m : Type -> Type) (a : Type) : Type := m (exn a).
+Set Universe Polymorphism.
 
+#[local]
+Close Scope nat_scope.
+#[local]
+Open Scope prelude_scope.
+
+(** * Definition *)
+
+Inductive exn(A:Type) : Type := 
+| Result : A -> exn A
+| Fail : string -> exn A.
+Arguments Result {A}.
+Arguments Fail {A}.
+
+Definition exn_map {a b} (f : a -> b) (r : exn a)
+  : (exn b):=
+match r with 
+| Result x => Result (f x)
+| Fail s => Fail s end.
+
+Definition exn_t  (m : Type -> Type) (a : Type) : Type := m (exn a).
+
+Bind Scope monad_scope with exn_t.
 
 Definition exn_t_map {m} `{Monad m} {a b} (f : a -> b) (r : exn_t m a)
-  : exn_t m b := 
-bind(m:=m) r (fun y => pure ((exn_map f) y)).
-                      
+  : exn_t m b := map (exn_map f) r.
+  
+  
 Lemma exn_t_functor_identity {m a} `{Monad m} 
   (r : exn_t m a)
   : exn_t_map id r = id r.
-Proof. unfold exn_t_map. 
-assert (H1: (fun y : exn a => pure (exn_map id y))= (fun (y: exn a)=> pure y)) by
-(apply functional_extensionality; intro; rewrite exn_functor_identity; auto).
 
-Admitted.
+
+Proof. unfold exn_t_map. assert (H1: exn_map(b:=a) id = id)
+by (apply functional_extensionality; intro x; destruct x; auto).
+rewrite H1. assert (H2: map(b:=exn a) id = id) by
+(apply functional_extensionality; intro x; apply  functor_identity).
+rewrite H2. trivial. Qed.
+
+Lemma exn_functor_composition_identity {a b c} 
+  (u : b -> c) (v : a -> b) (r : exn a)
+  : exn_map  (v >>> u) r = ((exn_map  v) >>> (exn_map  u)) r.
+Proof. unfold exn_map. destruct r; trivial. Qed.
+
+Lemma exn_t_functor_composition_identity {m a b c} `{Monad m} 
+  (u : b -> c) (v : a -> b) (r : exn_t  m a)
+  : exn_t_map (u <<< v) r = ((exn_t_map u) <<< (exn_t_map v)) r.
+Proof. unfold exn_t_map. assert (H1:  (exn_map (v>>>u)) = (exn_map v) >>> (exn_map u))
+by(apply functional_extensionality; intro; rewrite exn_functor_composition_identity; auto).
+rewrite H1. rewrite functor_map_identity. auto. Qed.
+
+#[program]
+Instance exn_t_Functor (m :  Type -> Type) `{Monad m} 
+  : Functor (exn_t m) :=
+  { map := @exn_t_map m  _
+  }.
+
+Next Obligation.
+  apply exn_t_functor_identity.
+Defined.
+
+Next Obligation.
+  apply exn_t_functor_composition_identity.
+Defined.
+
+Definition exn_apply{a b} (f : exn (a -> b)) (fs : exn a): exn b := 
+match fs with 
+| Fail s => Fail s
+| Result x => match f with 
+                | Result g => Result (g x)
+                | Fail t => Fail t end end .
+
+Definition exn_t_pure {m} `{Monad m} {a} (x : a) : exn_t m a := pure (Result x).
+
